theories/ftlr/WriteSR.v
@@ -1,0 +1,101 @@
+From cap_machine Require Export logrel.
+From iris.proofmode Require Import proofmode.
+From iris.program_logic Require Import weakestpre adequacy lifting.
+From stdpp Require Import base.
+From cap_machine.ftlr Require Import ftlr_base interp_weakening.
+From cap_machine.rules Require Import rules_base rules_WriteSR.
+From cap_machine.proofmode Require Import map_simpl register_tactics.
+From cap_machine Require Import stdpp_extra.
+
+Section fundamental.
+  Context
+    {Σ : gFunctors}
+      {ceriseg: ceriseG Σ}
+      {stsg : STSG Addr region_type Σ} {heapg : heapGS Σ}
+      {sealsg: sealStoreG Σ}
+      {nainv: logrel_na_invs Σ}
+      {MP: MachineParameters}
+  .
+
+  Notation STS := (leibnizO (STS_states * STS_rels)).
+  Notation STS_STD := (leibnizO (STS_std_states Addr region_type)).
+  Notation WORLD := (prodO STS_STD STS).
+  Implicit Types W : WORLD.
+
+  Notation D := (WORLD -n> (leibnizO Word) -n> iPropO Σ).
+  Notation R := (WORLD -n> (leibnizO Reg) -n> iPropO Σ).
+  Implicit Types w : (leibnizO Word).
+  Implicit Types interp : (D).
+
+   Lemma writesr_case (W : WORLD) (regs : leibnizO Reg)
+     (p p' : Perm) (g : Locality) (b e a : Addr)
+     (w : Word) (ρ : region_type) (dst : SRegName) (src : RegName) (P:D):
+    ftlr_instr W regs p p' g b e a w (WriteSR dst src) ρ P.
+  Proof.
+    intros Hp Hsome HcorrectPC Hbae Hfp HO Hpers Hpwl Hregion Hnotrevoked Hnotfrozen Hi.
+    iIntros "#IH #Hinv_interp #Hreg #Hinva #Hrcond #Hwcond #Hmono #HmonoV Hw Hsts Hown".
+    iIntros "Hr Hstate Ha HPC Hmap".
+    iInsert "Hmap" PC.
+    iApply (wp_WriteSR with "[$Ha $Hmap]"); eauto.
+    { simplify_map_eq; auto. }
+    { rewrite /subseteq /map_subseteq. intros rr _.
+      apply elem_of_dom. apply lookup_insert_is_Some'; eauto. }
+
+    iIntros "!>" (regs' retv). iDestruct 1 as (HSpec) "[Ha Hmap]".
+    destruct HSpec; cycle 1.
+    - iApply wp_pure_step_later; auto. iNext; iIntros "_".
+      iApply wp_value; auto. iIntros; discriminate.
+    - incrementPC_inv; simplify_map_eq.
+      rename x into p0
+      ; rename x0 into g0
+      ; rename x1 into b0
+      ; rename x2 into e0
+      ; rename x3 into a0
+      ; rename x4 into a0'.
+      iApply wp_pure_step_later; auto; iNext; iIntros "_".
+
+      destruct (decide (dst = PC)) as [HdstPC|HdstPC]; simplify_map_eq.
+      { map_simpl "Hmap".
+        destruct src; simpl in *; try discriminate.
+        iDestruct (region_close with "[$Hstate $Hr $Ha $HmonoV Hw]") as "Hr"; eauto.
+        { destruct ρ;auto;[|ospecialize (Hnotfrozen _)];contradiction. }
+        destruct (decide (r = PC)).
+        { simplify_map_eq.
+          iApply ("IH" $! _ regs with "[%] [] [Hmap] [$Hr] [$Hsts] [$Hown]"); eauto.
+          iApply (interp_next_PC with "Hinv_interp"); eauto.
+        }
+        simplify_map_eq.
+        iDestruct ("Hreg" $! r (WCap p0 g0 b0 e0 a0) n H ) as "Hr0".
+        destruct (executeAllowed p0) eqn:Hpft; cycle 1.
+        { iApply (wp_bind (fill [SeqCtx])).
+          iExtract "Hmap" PC as "HPC".
+          iApply (wp_notCorrectPC with "HPC"); [eapply not_isCorrectPC_perm; naive_solver|].
+          iNext; iIntros "HPC /=".
+          iApply wp_pure_step_later; auto; iNext; iIntros "_".
+          iApply wp_value; iIntros; discriminate.
+        }
+
+        iApply ("IH" $! _ regs with "[%] [] [Hmap] [$Hr] [$Hsts] [$Hown]"); eauto.
+        iApply (interp_weakening with "IH Hr0"); eauto; try reflexivity; try solve_addr.
+        by apply executeAllowed_nonSentry.
+      }
+      { map_simpl "Hmap".
+        iDestruct (region_close with "[$Hstate $Hr $Ha $HmonoV Hw]") as "Hr"; eauto.
+        { destruct ρ;auto;[|ospecialize (Hnotfrozen _)];contradiction. }
+        iApply ("IH" $! _ (<[dst:=w0]> _) with "[%] [] [Hmap] [$Hr] [$Hsts] [$Hown]"); eauto.
+        - intros; simpl.
+          rewrite lookup_insert_is_Some.
+          destruct (decide (dst = x)); auto; right; split; auto.
+        - iIntros (ri wi Hri Hregs_ri).
+          destruct (decide (ri = dst)); simplify_map_eq.
+          + (* ri = dst *)
+            destruct src; simplify_map_eq.
+            * repeat rewrite fixpoint_interp1_eq; auto.
+            * destruct (decide (PC = r)); simplify_map_eq; first done.
+              iApply ("Hreg" $! r) ; auto.
+          + iApply ("Hreg" $! ri) ; auto.
+      - iApply (interp_next_PC with "Hinv_interp"); eauto.
+      }
+  Qed.
+
+End fundamental.
