theories/rules.v
@@ -4,7 +4,8 @@ From cap_machine.rules Require Export
      rules_Get rules_Load rules_Store rules_AddSubLt
      rules_Lea rules_Mov rules_Restrict
      rules_Jmp rules_Jnz rules_Subseg
-     rules_Seal rules_UnSeal.
+     rules_Seal rules_UnSeal
+     rules_ReadSR rules_WriteSR.
 
 (* Program specifications
 
