theories/rules/rules_Lea.v
@@ -86,8 +86,7 @@ Section cap_lang_rules.
    Proof.
      iIntros (Hinstr Hvpc HPC Dregs φ) "(>Hpc_a & >Hmap) Hφ".
      iApply wp_lift_atomic_base_step_no_fork; auto.
-     iIntros (σ1 ns l1 l2 nt) "Hσ1 /=". destruct σ1; simpl.
-     iDestruct "Hσ1" as "[Hr Hm]".
+    iIntros (σ1 ns l1 l2 nt) "[ [Hr Hsr] Hm ] /=". destruct σ1 as [ [r sr] m]; cbn.
      iDestruct (gen_heap_valid_inclSepM with "Hr Hmap") as %Hregs.
      pose proof (lookup_weaken _ _ _ _ HPC Hregs).
      iDestruct (@gen_heap_valid with "Hm Hpc_a") as %Hpc_a; auto.
@@ -110,7 +109,7 @@ Section cap_lang_rules.
        odestruct (Hri r0) as [r0v [Hr'0 Hr0]].
        { unfold regs_of_argument. set_solver+. }
        rewrite Hr0 Hr'0 in Harg Hstep.
-       assert (c = Failed ∧ σ2 = (r, m)) as (-> & ->).
+       assert (c = Failed ∧ σ2 = (r, sr, m)) as (-> & ->).
        { destruct_word r0v; cbn in Hstep; try congruence; by simplify_pair_eq. }
        iFailWP "Hφ" Lea_fail_rv_nonconst. }
      apply (z_of_arg_mono _ r) in Harg; auto. rewrite Harg in Hstep; cbn in Hstep.
@@ -118,7 +117,7 @@ Section cap_lang_rules.
      destruct (is_mutable_range r1v) eqn:Hr1v.
      2: { (* Failure: r1v is not of the right type *)
        unfold is_mutable_range in Hr1v.
-       assert (c = Failed ∧ σ2 = (r, m)) as (-> & ->).
+       assert (c = Failed ∧ σ2 = (r, sr, m)) as (-> & ->).
        { destruct r1v as [ | [p b e a | ] | ]; try by inversion Hr1v.
          all: try by simplify_pair_eq.
          destruct_perm p; cbn in *; try congruence.
@@ -136,7 +135,7 @@ Section cap_lang_rules.
 
        destruct (a + argz)%a as [ a' |] eqn:Hoffset; cycle 1.
        { (* Failure: offset is too large *)
-         assert (c = Failed ∧ σ2 = (r, m)) as (-> & ->)
+         assert (c = Failed ∧ σ2 = (r, sr, m)) as (-> & ->)
              by (destruct p; inversion Hstep; auto).
          iFailWP "Hφ" Lea_fail_overflow_cap. }
 
@@ -148,13 +147,13 @@ Section cap_lang_rules.
          { eapply incrementPC_overflow_mono; first eapply Hregs'.
              by rewrite lookup_insert_is_Some'; eauto.
                by apply insert_mono; eauto. }
-         apply (incrementPC_fail_updatePC _ m) in HH. rewrite HH in Hstep.
-         assert (c = Failed ∧ σ2 = (r, m)) as (-> & ->)
+         apply (incrementPC_fail_updatePC _ sr m) in HH. rewrite HH in Hstep.
+         assert (c = Failed ∧ σ2 = (r, sr, m)) as (-> & ->)
              by (destruct p; inversion Hstep; auto).
          iFailWP "Hφ" Lea_fail_overflow_PC_cap. }
 
        (* Success *)
-       eapply (incrementPC_success_updatePC _ m) in Hregs'
+       eapply (incrementPC_success_updatePC _ sr m) in Hregs'
          as (p' & g' & b' & e' & a'' & a''' & a_pc' & HPC'' & HuPC & ->).
        eapply updatePC_success_incl in HuPC. 2: by eapply insert_mono; eauto.
        rewrite HuPC in Hstep; clear HuPC.
@@ -170,7 +169,7 @@ Section cap_lang_rules.
     (* Now, the case where r1v is a sealrange *)
      + destruct (a + argz)%ot as [ a' |] eqn:Hoffset; cycle 1.
        { (* Failure: offset is too large *)
-         assert (c = Failed ∧ σ2 = (r, m)) as (-> & ->)
+         assert (c = Failed ∧ σ2 = (r, sr, m)) as (-> & ->)
              by (destruct p; inversion Hstep; auto).
          iFailWP "Hφ" Lea_fail_overflow_sr. }
 
@@ -182,13 +181,13 @@ Section cap_lang_rules.
          { eapply incrementPC_overflow_mono; first eapply Hregs'.
              by rewrite lookup_insert_is_Some'; eauto.
                by apply insert_mono; eauto. }
-         apply (incrementPC_fail_updatePC _ m) in HH. rewrite HH in Hstep.
-         assert (c = Failed ∧ σ2 = (r, m)) as (-> & ->)
+         apply (incrementPC_fail_updatePC _ sr m) in HH. rewrite HH in Hstep.
+         assert (c = Failed ∧ σ2 = (r, sr, m)) as (-> & ->)
              by (destruct p; inversion Hstep; auto).
          iFailWP "Hφ" Lea_fail_overflow_PC_sr. }
 
        (* Success *)
-       eapply (incrementPC_success_updatePC _ m) in Hregs'
+       eapply (incrementPC_success_updatePC _ sr m) in Hregs'
          as (p' & g' & b' & e' & a'' & a''' & a_pc' & HPC'' & HuPC & ->).
        eapply updatePC_success_incl in HuPC. 2: by eapply insert_mono; eauto.
        rewrite HuPC in Hstep; clear HuPC.
