theories/rules/rules_Restrict.v
@@ -106,8 +106,7 @@ Section cap_lang_rules.
   Proof.
     iIntros (Hinstr Hvpc HPC Dregs φ) "(>Hpc_a & >Hmap) Hφ".
     iApply wp_lift_atomic_base_step_no_fork; auto.
-    iIntros (σ1 ns l1 l2 nt) "Hσ1 /=". destruct σ1; simpl.
-    iDestruct "Hσ1" as "[Hr Hm]".
+    iIntros (σ1 ns l1 l2 nt) "[ [Hr Hsr] Hm ] /=". destruct σ1 as [ [r sr] m]; cbn.
     iDestruct (gen_heap_valid_inclSepM with "Hr Hmap") as %Hregs.
     have ? := lookup_weaken _ _ _ _ HPC Hregs.
     iDestruct (@gen_heap_valid with "Hm Hpc_a") as %Hpc_a; auto.
@@ -130,7 +129,7 @@ Section cap_lang_rules.
        odestruct (Hri r0) as [r0v [Hr'0 Hr0]].
        { unfold regs_of_argument. set_solver+. }
        rewrite Hr0 Hr'0 in Hwsrc Hstep.
-       assert (c = Failed ∧ σ2 = (r, m)) as (-> & ->).
+       assert (c = Failed ∧ σ2 = (r, sr, m)) as (-> & ->).
        { destruct_word r0v; cbn in Hstep; try congruence; by simplify_pair_eq. }
        iFailWP "Hφ" Restrict_fail_src_nonz. }
     apply (z_of_arg_mono _ r) in Hwsrc; auto. rewrite Hwsrc in Hstep; simpl in Hstep.
@@ -138,7 +137,7 @@ Section cap_lang_rules.
     destruct (is_mutable_range wdst) eqn:Hwdst.
      2: { (* Failure: wdst is not of the right type *)
        unfold is_mutable_range in Hwdst.
-       assert (c = Failed ∧ σ2 = (r, m)) as (-> & ->).
+       assert (c = Failed ∧ σ2 = (r, sr, m)) as (-> & ->).
        { destruct wdst as [ | [p b e a | ] | ]; try by inversion Hwdst.
          all: try by simplify_pair_eq.
          destruct_perm p; cbn in *; try congruence.
@@ -170,14 +169,14 @@ Section cap_lang_rules.
          { eapply incrementPC_overflow_mono; first eapply Hregs'.
              by rewrite lookup_insert_is_Some'; eauto.
                by apply insert_mono; eauto. }
-         apply (incrementPC_fail_updatePC _ m) in HH. rewrite HH in Hstep.
-         assert (c = Failed ∧ σ2 = (r, m)) as (-> & ->)
+         apply (incrementPC_fail_updatePC _ sr m) in HH. rewrite HH in Hstep.
+         assert (c = Failed ∧ σ2 = (r, sr, m)) as (-> & ->)
              by (destruct p; inversion Hstep; auto).
          iFailWP "Hφ" Restrict_fail_PC_overflow_cap. }
 
-       eapply (incrementPC_success_updatePC _ m) in Hregs'
+       eapply (incrementPC_success_updatePC _ sr m) in Hregs'
          as (p'' & g'' & b' & e' & a'' & a''' & a_pc' & HPC'' & HuPC & ->).
-       eapply updatePC_success_incl with (m':=m) in HuPC. 2: by eapply insert_mono; eauto. rewrite HuPC in Hstep.
+       eapply updatePC_success_incl with (sregs':=sr) (m':=m) in HuPC. 2: by eapply insert_mono; eauto. rewrite HuPC in Hstep.
        eassert ((c, σ2) = (NextI, _)) as HH.
        { destruct_perm p; cbn in *; eauto. }
        simplify_pair_eq.
@@ -205,14 +204,14 @@ Section cap_lang_rules.
          { eapply incrementPC_overflow_mono; first eapply Hregs'.
              by rewrite lookup_insert_is_Some'; eauto.
                by apply insert_mono; eauto. }
-         apply (incrementPC_fail_updatePC _ m) in HH. rewrite HH in Hstep.
-         assert (c = Failed ∧ σ2 = (r, m)) as (-> & ->)
+         apply (incrementPC_fail_updatePC _ sr m) in HH. rewrite HH in Hstep.
+         assert (c = Failed ∧ σ2 = (r, sr, m)) as (-> & ->)
              by (destruct p; inversion Hstep; auto).
          iFailWP "Hφ" Restrict_fail_PC_overflow_sr. }
 
-       eapply (incrementPC_success_updatePC _ m) in Hregs'
+       eapply (incrementPC_success_updatePC _ sr m) in Hregs'
          as (p'' & g'' & b' & e' & a'' & a''' & a_pc' & HPC'' & HuPC & ->).
-       eapply updatePC_success_incl with (m':=m) in HuPC. 2: by eapply insert_mono; eauto. rewrite HuPC in Hstep.
+       eapply updatePC_success_incl with (sregs':=sr) (m':=m) in HuPC. 2: by eapply insert_mono; eauto. rewrite HuPC in Hstep.
        eassert ((c, σ2) = (NextI, _)) as HH.
        { destruct p; cbn in Hstep; eauto. }
        simplify_pair_eq.
